finished p4cub climate

deps/poulet4/lib/P4cub/Semantics/Climate.v
@@ -1,6 +1,5 @@
-Require Import Poulet4.Utils.Util.Utiliser.
-
-Declare Custom Entry p4env.
+Require Import Poulet4.Utils.Util.Utiliser
+        Coq.Logic.FunctionalExtensionality.
 
 (** * Environments *)
 Module Clmt.
@@ -43,9 +42,15 @@ Module Clmt.
         (e₂ k <> None -> e₁ k = None).
     
     Definition union (e₁ e₂ : t D T) : t D T :=
-      fun y => match e₁ y, e₂ y with
-            | Some v, _ | _, Some v => Some v
-            | _, _ => None
+      fun y => match e₁ y with
+            | Some v => Some v
+            | None   => e₂ y
+            end.
+
+    Definition strip (e₁ e₂ : t D T) : t D T :=
+      fun y => match e₁ y with
+            | Some _ => None
+            | None   => e₂ y
             end.
     
     Definition disjoint_union (e₁ e₂ e₃ : t D T) : Prop :=
@@ -91,37 +96,30 @@ Module Clmt.
       Global Instance sub_env_antisymmetric
         : @Antisymmetric _ eq _ sub_env.
       Proof.
-        unfold Antisymmetric.
-      Admitted.
+        unfold Antisymmetric, sub_env.
+        intros e1 e2 H1 H2.
+        extensionality k.
+        destruct (e2 k) as [v2 |] eqn:He2; auto.
+        destruct (e1 k) as [v1 |] eqn:He1; auto.
+        apply H1 in He1; rewrite He2 in He1; discriminate.
+      Qed.
 
       (** TODO: [e ⊆ bind k v e <-> find k e = None \/ find k e = Some v] *)
       Lemma find_none_bind_sub_env : forall e k v,
-          find k e = None -> sub_env e (bind k v e).
+          e k = None -> sub_env e (bind k v e).
       Proof.
         unfold sub_env, bind;
           intros e k v H k' v' Hkv'; simpl.
-        destruct_if; auto.
-        assert (Hfind: find k' e = find k e)
-          by auto using find_equiv_rel.
-        rewrite Hfind, H in Hkv'; discriminate.
+        destruct_if; auto; subst.
+        rewrite H in Hkv'; discriminate.
       Qed.
       
-      Lemma bind_sub_env_find_none : forall e k v,
-          sub_env e (bind k v e) ->
-          find k e = None \/ find k e = Some v.
+      Lemma union_sub_env :
+        forall e1 e2, sub_env e1 (union e1 e2).
       Proof.
-        unfold sub_env, bind;
-          intro e; induction e as [| [d t] e IHe]; simpl in *;
-            intros ky vl H; auto.
-      Abort.
-      
-      Lemma scope_shadow_sub_env :
-        forall e1 e2, sub_env e1 (scope_shadow e1 e2).
-      Proof.
-        unfold sub_env, scope_shadow;
+        unfold sub_env, union;
           intros e1 e2 k v Hkv.
-        induction e1 as [| [k1 v1] e1 IHe1];
-          simpl in *; auto; try discriminate.
+        rewrite Hkv; reflexivity.
       Qed.
       
       Lemma disjoint_sym : forall e1 e2,
@@ -137,12 +135,13 @@ Module Clmt.
       Qed.
       
       Lemma disjoint_nexists : forall e1 e2,
-          disjoint e1 e2 -> ~ exists k v, find k e1 = Some v /\ find k e2 = Some v.
+          disjoint e1 e2 ->
+          ~ exists k v, e1 k = Some v /\ e2 k = Some v.
       Proof.
         intros e1 e2 H (k & v & He1 & He2).
         unfold disjoint in H; specialize H with k.
         destruct H as [H1 H2].
-        assert (Hnone: find k e1 <> None).
+        assert (Hnone: e1 k <> None).
         { rewrite He1; discriminate. }
         apply H1 in Hnone. rewrite Hnone in He2.
         discriminate.
@@ -151,255 +150,175 @@ Module Clmt.
       (** Need assumption that [e1]
           and [e2] are not empty. *)
       Lemma disjoint_eq_env : forall e1 e2,
-          disjoint e1 e2 -> ~ eq_env e1 e2.
+          disjoint e1 e2 -> e1 <> e2.
       Proof.
-        unfold disjoint, eq_env, sub_env.
-        intros e1 e2 Hd [Hs1 Hs2].
+        unfold disjoint; intros e1 e2 Hd H; subst.
+        apply forall_conj_distr in Hd.
+        destruct Hd as [H1 _].
       Abort.
-      
-      Lemma find_app_eq : forall e1 e2 k,
-          find k (e1 ++ e2) =
-          match find k e1 with
-          | Some v => Some v
-          | None   => find k e2
-          end.
+            
+      Lemma find_union_l : forall e1 e2 k v,
+          e1 k = Some v ->
+          union e1 e2 k = Some v.
       Proof.
-        intros e1; induction e1 as [| [k1 v1] e1 IHe1];
-          intros e2 k; unravel; auto.
-        destruct_if; auto.
+        intros e1 e2 k v H; unfold union;
+          rewrite H; reflexivity.
       Qed.
       
-      Lemma find_app_l : forall e1 e2 k v,
-          find k e1 = Some v ->
-          find k (e1 ++ e2) = Some v.
+      Local Hint Resolve find_union_l : core.
+      
+      Lemma find_union_r : forall e1 e2 k,
+          e1 k = None ->
+          union e1 e2 k = e2 k.
       Proof.
-        intros e1 e2 k v H; rewrite find_app_eq, H; reflexivity.
+        unfold union; intros e1 e2 k H; rewrite H; reflexivity.
+      Qed.
+
+      Local Hint Resolve find_union_r : core.
+      
+      Lemma find_union_some : forall e1 e2 k v,
+          union e1 e2 k = Some v ->
+          e1 k = Some v \/ e2 k = Some v.
+      Proof.
+        intros e1 e2 k v H; unfold union in *.
+        destruct (e1 k) as [v1 |] eqn:Hke1; auto.
+      Qed.
+
+      Local Hint Resolve find_union_some : core.
+      
+      Lemma disjoint_union_eq_env : forall e1 e2,
+          disjoint e1 e2 -> union e1 e2 = union e2 e1.
+      Proof.
+        unfold disjoint; intros e1 e2 H.
+        extensionality k.
+        unfold disjoint. apply forall_conj_distr in H as [H1 H2].
+        specialize H1 with k; specialize H2 with k.
+        unfold union.
+        destruct (e1 k) as [v1 |] eqn:He1;
+          destruct (e2 k) as [v2 |] eqn:He2; auto;
+            assert (Hneq: Some v1 <> None) by discriminate;
+            apply H1 in Hneq; discriminate.
       Qed.
       
-      Lemma find_app_r : forall e1 e2 k,
-          find k e1 = None ->
-          find k (e1 ++ e2) = find k e2.
-      Proof.
-        intros e1 e2 k H; rewrite find_app_eq, H; reflexivity.
-      Qed.
-      
-      Lemma find_app_some : forall e1 e2 k v,
-          find k (e1 ++ e2) = Some v ->
-          find k e1 = Some v \/ find k e2 = Some v.
-      Proof.
-        intros e1 e2 k v H.
-        rewrite find_app_eq in H.
-        destruct (find k e1) as [v1 |] eqn:Hke1; auto.
-      Qed.
-      
-      Lemma disjoint_append_eq_env : forall e1 e2,
-          disjoint e1 e2 -> eq_env (e1 ++ e2) (e2 ++ e1).
-      Proof.
-        unfold disjoint, eq_env, sub_env;
-          intros e1 e2 Hd; split; intros k v Hkv;
-            rewrite find_app_eq in *;
-            specialize Hd with k; destruct Hd as [Hd1 Hd2];
-              destruct (find k e1) as [v1 |] eqn:He1;
-              destruct (find k e2) as [v2 |] eqn:He2; auto;
-                assert (Hneq: Some v1 <> None) by discriminate;
-                apply Hd1 in Hneq; discriminate.
-      Qed.
-      
-      Lemma disjoint_nil : forall e, disjoint e [].
+      Lemma disjoint_empty : forall e, disjoint e (empty D T).
       Proof.
         unfold disjoint; intros e k; split;
           unravel; auto; try contradiction.
       Qed.
       
-      Local Hint Resolve disjoint_append_eq_env : core.
+      Local Hint Resolve disjoint_union_eq_env : core.
       Local Hint Resolve disjoint_sym : core.
       
       Lemma disjoint_union_sym : forall e1 e2 e3,
           disjoint_union e1 e2 e3 -> disjoint_union e2 e1 e3.
       Proof.
         unfold disjoint_union.
-        intros e1 e2 e3 [Hd Heq]; split; auto.
-        assert (eq_env (e1 ++ e2) (e2 ++ e1)) by auto.
-        etransitivity; eauto.
+        intros e1 e2 e3 [Hd Heq]; split; subst; auto.
       Qed.
       
-      Lemma disjoint_sub_env_app_inj_r : forall l r r',
+      Lemma disjoint_sub_env_union_inj_r : forall l r r',
           disjoint l r ->
-          sub_env (l ++ r) (l ++ r') -> sub_env r r'.
+          sub_env (union l r) (union l r') -> sub_env r r'.
       Proof.
         unfold disjoint, sub_env; intros l r r' Hd Hs k v Hkv;
           specialize Hd with k; specialize Hs with k v;
             destruct Hd as [Hd1 Hd2].
-        assert (Hnone: find k r <> None) by (rewrite Hkv; discriminate).
+        assert (Hnone: r k <> None) by (rewrite Hkv; discriminate).
         apply Hd2 in Hnone.
-        repeat rewrite find_app_eq, Hnone in Hs; auto.
+        assert (union l r k = Some v) by (rewrite <- Hkv; auto).
+        apply Hs in H. apply find_union_some in H.
+        destruct H as [H | H];
+          try rewrite H in Hnone; auto; discriminate.
       Qed.
       
-      Lemma eq_env_disjoint : forall e1 e2 e3,
-          eq_env e1 e2 -> disjoint e1 e3 -> disjoint e2 e3.
-      Proof.
-        unfold eq_env, sub_env, disjoint;
-          intros e1 e2 e3 [Hs1 Hs2] Hd k;
-          specialize Hs1 with (k := k); specialize Hs2 with (k := k);
-            specialize Hd with k; destruct Hd as [Hd1 Hd2]; split; intros H.
-        - apply Hd1.
-          destruct (find k e2) as [v2 |] eqn:Hv2; try contradiction.
-          assert (Hke1: find k e1 = Some v2) by auto.
-          rewrite Hke1; discriminate.
-        - apply Hd2 in H.
-          destruct (find k e2) as [v2 |] eqn:Hv2; auto.
-          assert (Hke1 : find k e1 = Some v2) by auto.
-          rewrite Hke1 in H; discriminate.
-      Qed.
-      
-      Local Hint Resolve disjoint_sub_env_app_inj_r : core.
-      
-      Lemma eq_env_app_inj : forall l r r',
+      Lemma eq_env_union_inj : forall l r r',
           disjoint l r -> disjoint l r' ->
-          eq_env (l ++ r) (l ++ r') -> eq_env r r'.
+          union l r = union l r' -> r = r'.
       Proof.
-        unfold eq_env; intuition; eauto.
+        unfold disjoint; intros l r r' Hr Hr' Hu.
+        extensionality k.
+        specialize Hr with k; specialize Hr' with k.
+        destruct Hr as [Hlr Hrl]; destruct Hr' as [Hlr' Hrl'].
+        apply equal_f with k in Hu.
+        unfold union in Hu.
+        destruct (l k) as [v |] eqn:Hlk; auto.
+        assert (Hneq: Some v <> None) by discriminate.
+        pose proof Hlr Hneq as Hrk;
+          pose proof Hlr' Hneq as Hrk';
+          rewrite Hrk, Hrk'; reflexivity.
       Qed.
       
-      Local Hint Resolve eq_env_app_inj : core.
+      Local Hint Resolve eq_env_union_inj : core.
       
       Lemma disjoint_union_unique_eq_env_r : forall l r r' e,
           disjoint_union l r e ->
-          disjoint_union l r' e -> eq_env r r'.
+          disjoint_union l r' e -> r = r'.
       Proof.
         unfold disjoint_union.
-        intros l r r' e [Hdr Hr] [Hdr' Hr'].
-        assert (Hlrr': eq_env (l ++ r) (l ++ r')).
-        { symmetry in Hr'; transitivity e; auto. }
+        intros l r r' e [Hdr Hr] [Hdr' Hr']; subst.
         eauto.
       Qed.
       
       Lemma disjoint_union_unique_eq_env :  forall l r e e',
           disjoint_union l r e ->
-          disjoint_union l r e' -> eq_env e e'.
+          disjoint_union l r e' -> e = e'.
       Proof.
-        unfold disjoint_union; firstorder.
+        unfold disjoint_union;
+          intros l r e e' [Hd He] [Hd' He'];
+          subst; reflexivity.
       Qed.
       
-      Lemma app_sub_env : forall e1 e2 e3,
-          sub_env (e1 ++ e2) e3 -> sub_env e1 e3.
+      Lemma sub_env_union : forall e1 e2 e3,
+          sub_env (union e1 e2) e3 -> sub_env e1 e3.
       Proof.
-        unfold sub_env; intros e1 e2 e3 H k v Hkv;
-        specialize H with k v.
-      rewrite find_app_eq, Hkv in H; auto.
-    Qed.
+        unfold sub_env; intros e1 e2 e3 H k v Hkv; eauto.
+      Qed.
 
-    Local Hint Resolve app_sub_env : core.
+      Local Hint Resolve sub_env_union : core.
+      Local Hint Resolve union_sub_env : core.
+      
+      Lemma disjoint_union_sub_env : forall e1 e2 e3,
+          disjoint_union e1 e2 e3 -> sub_env e1 e3.
+      Proof.
+        intros e1 e2 e3 [Hd He3]; subst; auto.
+      Qed.
+      
+      Local Hint Resolve disjoint_empty : core.
+      Local Hint Resolve disjoint_sym : core.
     
-    Lemma disjoint_union_sub_env : forall e1 e2 e3,
-        disjoint_union e1 e2 e3 -> sub_env e1 e3.
-    Proof.
-      unfold disjoint_union, eq_env; intuition; eauto.
-    Qed.
+      Lemma sub_env_disjoint_union_exists : forall e1 e2,
+          sub_env e1 e2 -> exists e, disjoint_union e1 e e2.
+      Proof.
+        intros e1 e2 Hs.
+        unfold disjoint_union.
+        exists (strip e1 e2).
+        (* TODO: helper lemmas. *)
+      Admitted.
+    End Lemmas.
+  End EnvDefs.
 
-    Lemma sub_env_bind_l : forall l r k v,
-        sub_env ((k,v) :: l) r <->
-        find k r = Some v /\
-        match find k l with
-        | None    => sub_env l r
-        | Some v' => (v = v' /\ sub_env l r) \/ False (* TODO? *)
-        end.
-    Abort.
-    
-    Local Hint Resolve disjoint_nil : core.
-    Local Hint Resolve disjoint_sym : core.
-    
-    Lemma sub_env_bind_r : forall l r k v,
-        sub_env l (bind k v r) ->
-        sub_env l r \/ find k l = Some v.
-    Proof.
-      unfold sub_env, bind.
-      intro l; induction l as [| [kl vl] l IHl];
-        intros r k v Hs.
-      - left; intros ks vs Hksvs; simpl in *; discriminate.
-      - specialize IHl with r k v; unravel in *.
-        destruct_if.
-    Abort.
-    
-    Lemma sub_env_disjoint_union_exists : forall e1 e2,
-        sub_env e1 e2 -> exists e, disjoint_union e1 e e2.
-    Proof.
-      intros e1 e2 Hs.
-      unfold disjoint_union.
-      induction e1 as [| [k1 v1] e1 IHe1].
-      - firstorder.
-      - (* need unique representation maybe
-           for proof. *)
-    Admitted.
-  End Lemmas.
-End EnvDefs.
-
-Section MapKeys.
-  Context {A B T : Type}.
-  Variable (f : A -> B).
+  Section MapVals.
+    Context {D U V : Type}.
+    Variable (f : U -> V).
   
-  Definition map_keys : t A T -> t B T :=
-    List.map (fun '(k, v) => (f k, v)).
+    Definition map_vals (e : t D U) : t D V :=
+      fun k => e k >>| f.
+  End MapVals.
 
-  Context {EA : EqDec A eq}.
-  Context {EB : EqDec B eq}.
-  Hypothesis Hfinj : forall a1 a2, f a1 = f a2 -> a1 = a2.
-
-  Local Hint Extern 0 => simpl_equiv_dec : core.
-  Local Hint Extern 0 => simpl_equiv_dec_hyp : core.
-  
-  Lemma map_keys_find_injective : forall e a,
-      find (f a) (map_keys e) = find a e.
-  Proof.
-    intro e;
-      induction e as [| [k v] e IHe];
-      intros a; unravel in *; try reflexivity.
-    repeat (destruct_if; auto);
-      subst; intuition.
-  Qed.
-End MapKeys.
-
-Section MapVals.
-  Context {D U V : Type}.
-  Variable (f : U -> V).
-  
-  Definition map_vals : t D U -> t D V :=
-    List.map (fun '(k, v) => (k, f v)).
-
-  Context {R : D -> D -> Prop}.
-  Context {RE: Equivalence R}.
-  Context {RED: EqDec D R}.
-
-  Local Hint Extern 0 => simpl_equiv_dec : core.
-  Local Hint Extern 0 => simpl_equiv_dec_hyp : core.
-
-  Lemma map_vals_find : forall e d,
-      find d (map_vals e) = find d e >>| f.
-  Proof.
-    intro e;
-      induction e as [| [k u] e IHe];
-      intros d; unravel in *; try reflexivity;
-        repeat (destruct_if; auto).
-  Qed.
-End MapVals.
-
-Module EnvNotations.
-  Notation "e1 '⊆' e2"
-    := (sub_env e1 e2)
-         (at level 80, no associativity) : type_scope.
-  Notation "e1 '≝' e2"
-    := (eq_env e1 e2)
-         (at level 80, no associativity) : type_scope.
-  Notation "'!{' env '}!'" := env (env custom p4env at level 99).
-  Notation "x" := x (in custom p4env at level 0, x constr at level 0).
-  Notation "'∅'" := (empty _ _) (in custom p4env at level 0, no associativity).
-  Notation "x ↦ v ';;' e"
-    := (bind x v e)
-         (in custom p4env at level 40, e custom p4env,
-             right associativity).
-  Notation "e1 ≪ e2"
-           := (scope_shadow e1 e2)
-                (in custom p4env at level 41, e1 custom p4env,
-                    e2 custom p4env, right associativity).
-End EnvNotations.
+  Module Notations.
+    Declare Scope climate_scope.
+    Delimit Scope climate_scope with climate.
+    
+    Notation "e1 '⊆' e2"
+      := (sub_env e1 e2)
+           (at level 80, no associativity) : type_scope.
+    Notation "'∅'"
+      := (empty _ _) (at level 0, no associativity) : climate_scope.
+    Notation "x ↦ v ';;' e"
+      := (bind x v e)
+           (at level 41, right associativity) : climate_scope.
+    Notation "e1 ≪ e2"
+      := (shadow e1 e2)
+           (at level 41, right associativity) : climate_scope.
+  End Notations.
 End Clmt.
